

# PSTAT160A Stochastic Processes

## Section 6 - Solutions

**Authors:** Denisse Alejandra Escobar Parra, John Inston

**Date:** November 18, 2025

---

### Problem 1 - Dobrow 4.3

Let  $X \sim \text{Poisson}(\lambda)$  and  $Y \sim \text{Poisson}(\mu)$ . Assume that  $X$  and  $Y$  are independent. Use PGFs to find the distribution of  $X + Y$ .

#### Solution

The PGF of a random variable following a *Poisson Distribution* with rate  $\lambda$  is given by

$$M_X(s) := \mathbb{E}[s^X] = \exp(\lambda(s - 1)).$$

Since  $X$  and  $Y$  are independent we have that

$$\begin{aligned} M_{X+Y}(s) &= M_X(s) \cdot M_Y(s) \\ &= \exp(\lambda(s - 1)) \cdot \exp(\mu(s - 1)) \\ &= \exp((\lambda + \mu)(s - 1)). \end{aligned}$$

This is the MGF of a Poisson random variable with rate  $\lambda + \mu$  which is therefore the distribution of  $X + Y$  since the MGF uniquely determines the distribution.

### Problem 2 - Dobrow 4.4

If  $X$  has a *Negative Binomial Distribution* with parameters  $r$  and  $p$ , then  $X$  can be written as the sum of  $r$  i.i.d. *Geometric* random variables with parameter  $p$ . Use this fact to find the PGF of  $X$ . Then, use the PGF to find the mean and variance of the negative binomial distribution.

#### Solution

Define a sequence  $\{\xi_i\}_{i=1}^r$  of i.i.d. geometric random variables with PMF

$$p_{\xi_1}(k) := \mathbb{P}(\xi_1 = k) = (1 - p)^{k-1}p; \quad k \in \mathbb{N}_0,$$

The PGF is given by

$$G_{\xi_1}(s) = \mathbb{E}[s^{\xi_1}] = \frac{p}{1 - s + ps}.$$

From the independence of  $\xi_i$  we can therefore compute  $X = \sum_{i=1}^r \xi_i = r\xi_1 \sim \text{NB}(r, p)$  and the associated PGF

$$\begin{aligned} G_X(s) &= G_{\sum_{i=1}^r \xi_i}(s) \\ &= (P_{\xi_1}(s))^r \\ &= \left( \frac{p}{1-s+ps} \right)^r. \end{aligned}$$

The expectation is given by

$$\mathbb{E}[X] = G_X^{(1)}(0),$$

hence we first apply the Chain Rule to compute

$$\begin{aligned} G_X^{(1)}(s) &= \frac{d}{ds} \left( \frac{p}{1-(1-p)s} \right)^r \\ &= p^r \frac{d}{ds} \left( \frac{1}{1-(1-p)s} \right)^r \\ &= p^r r \left( \frac{1}{1-(1-p)s} \right)^{r-1} \cdot \frac{d}{ds} (1-(1-p)s)^{-1} \\ &= p^r r \left( \frac{1}{1-(1-p)s} \right)^{r-1} \cdot -(1-(1-p)s)^{-2} \cdot \frac{d}{ds} (1-(1-p)s) \\ &= p^r r \left( \frac{1}{1-(1-p)s} \right)^{r-1} \cdot -(1-(1-p)s)^{-2} \cdot -(1-p) \\ &= \frac{p^r r (1-p)}{(1-(1-p)s)^{r+1}}. \end{aligned}$$

Evaluating at  $s = 1$  we have that  $1 - (1-p) = p$  hence

$$\mathbb{E}[X] = \frac{r(1-p)}{p}.$$

Similarly, the variance is given by

$$\text{Var}(X) = G_X^{(2)}(1) + G_X^{(1)}(1) - [G_X^{(1)}(1)]^2,$$

therefore we again apply the Chain Rule to compute

$$\begin{aligned} G_X^{(2)}(s) &= \frac{d}{ds} \frac{p^r r (1-p)}{(1-(1-p)s)^{r+1}} \\ &= p^r r (1-p) \cdot \frac{d}{ds} (1-(1-p)s)^{-r-1} \\ &= p^r r (1-p) \cdot -(r+1)(1-(1-p)s)^{-r-2} \cdot \frac{d}{ds} (1-(1-p)s) \\ &= p^r r (1-p) \cdot -(r+1)(1-(1-p)s)^{-r-2} \cdot -(1-p) \\ &= \frac{p^r r (1-p)^2 (r+1)}{(1-(1-p)s)^{r+2}}. \end{aligned}$$

Evaluating at  $s = 1$  we obtain

$$\begin{aligned} G_X^{(2)}(1) &= \frac{p^r r(1-p)^2(r+1)}{p^{r+2}} \\ &= \frac{r(1-p)^2(r+1)}{p^2}. \end{aligned}$$

Substituting back into our expression we have

$$\begin{aligned} \text{Var}(X) &= \frac{r(r+1)(1-p)^2}{p^2} + \frac{r(1-p)}{p} - \left[ \frac{r(1-p)}{p} \right]^2 \\ &= \frac{r(r+1)(1-p)^2 + rp(1-p) - r^2(1-p)^2}{p^2} \\ &= \frac{r(1-p)\{(r+1)(1-p) + p - r(1-p)\}}{p^2} \\ &= \frac{r(1-p)\{r - rp - p + 1 + p - r + rp\}}{p^2} \\ &= \frac{r(1-p)}{p^2}. \end{aligned}$$

### Problem 3 - Dobrow 4.12

A branching process has offspring distribution  $\alpha = (\frac{1}{4}, \frac{1}{4}, \frac{1}{2})$ . Find the following:

1.  $\mu$ ;
2.  $G(s)$ ;
3. The extinction probability;
4.  $G_2(s)$ ; and
5.  $\mathbb{P}(Z_2 = 0)$ .

### Solution

Consider a branching process  $\{Z_n\}$  defined

$$Z_n := \sum_{i=1}^{Z_{n-1}} Z_{n,i},$$

where  $Z_{n,i}$  are i.i.d. with offspring distribution  $p_k = \mathbb{P}(Z_{n,i} = k)$  for  $k \in \mathbb{N}$  and  $Z_0 = 1$ . Specifically we have that

$$p_k = \begin{cases} \frac{1}{4} & k \in \{0, 1\} \\ \frac{1}{2} & k \in \{2\} \\ 0 & \text{o.w.} \end{cases}$$

(1) The mean of the offspring distribution is

$$\begin{aligned}
\mu &= \mathbb{E}[Z_{n,i}] \\
&= \sum_k k \cdot p_k \\
&= \frac{1}{4} + \frac{2}{2} \\
&= \frac{5}{4}.
\end{aligned}$$

(2) To find the generator of one offspring we compute

$$\begin{aligned}
G(s) &= \mathbb{E}[s^{Z_{n,i}}] \\
&= \sum_k p_k s^k \\
&= \frac{1}{4} + \frac{s}{4} + \frac{s^2}{2} \\
&= \frac{2s^2 + s + 1}{4}.
\end{aligned}$$

(3) To find the extinction probability  $\eta$  we solve

$$\begin{aligned}
\eta &= G(\eta) = \frac{2\eta^2 + \eta + 1}{4} \\
\Rightarrow 2\eta^2 - 3\eta + 1 &= 0 \\
\Rightarrow (2\eta - 1)(\eta - 1) &= 0,
\end{aligned}$$

hence  $\eta = \frac{1}{2}$  or  $\eta = 1$ . Since  $\mu > 1$  we have that  $\eta < 1$  thus  $\eta = \frac{1}{2}$ .

(4) We can compute

$$\begin{aligned}
G_2(s) &= G(G(s)) \\
&= \frac{1}{4}[2G^2(s) + G(s) + 1].
\end{aligned}$$

To avoid messy computations we first write

$$\begin{aligned}
G^2(s) &= \left( \frac{2s^2 + s + 1}{4} \right)^2 \\
&= \frac{4s^4 + 2s^3 + 2s^2 + 2s^3 + s^2 + s + 2s^2 + s + 1}{16} \\
&= \frac{4s^4 + 4s^3 + 5s^2 + 2s + 1}{16}.
\end{aligned}$$

Substituting back into our initial expression we find

$$\begin{aligned}
G_2(s) &= \left\{ \frac{\frac{4s^4 + 4s^3 + 5s^2 + 2s + 1}{8} + \frac{2s^2 + s + 1}{4} + 1}{4} \right\} \\
&= \frac{4s^4 + 4s^3 + 5s^2 + 2s + 1 + 4s^2 + 2s + s + 8}{32} \\
&= \frac{4s^4 + 4s^3 + 9s^2 + 4s + 11}{32}.
\end{aligned}$$

(5) To compute  $\mathbb{P}(Z_2 = 0)$  we have that

$$\begin{aligned}\mathbb{P}(Z_2 = 0) &= \frac{G_2^{(0)}(0)}{0!} \\ &= \frac{11}{32}.\end{aligned}$$

#### Problem 4 - Dobrow 4.18

Consider a branching process with offspring distribution

$$\alpha = (p^2, 2p(1-p), (1-p)^2); \quad 0 < p < 1.$$

The offspring distribution is binomial with parameters 2 and  $1-p$ . Find the extinction probability  $\eta$ .

#### Solution

Consider the new branching with offspring distribution

$$p_k = \begin{cases} p^2 & k = 0 \\ 2p(1-p) & k = 1 \\ (1-p)^2 & k = 2 \\ 0 & \text{o.w.} \end{cases}$$

First we compute

$$\begin{aligned}\mu &= 2p(1-p) + 2(1-p)^2 \\ &= 2p - 2p^2 + 2 - 4p + 2p^2 \\ &= 2 - 2p.\end{aligned}$$

Thus  $\mu = 2 - 2p > 1 \implies p < \frac{1}{2}$  is the supercritical case, otherwise  $\eta = 1$ . When  $p < \frac{1}{2}$  to find the extinction probability we first find the offspring generator as

$$\begin{aligned}G(s) &= \mathbb{E}[s^{Z_{n,i}}] \\ &= \sum_k s^k \cdot p_k \\ &= p^2 + 2ps(1-p) + s^2(1-p)^2 \\ &= p^2 + 2ps - 2p^2s + s^2 - 2ps^2 + s^2p^2.\end{aligned}$$

We can then compute the extinction probability by solving

$$\begin{aligned}\eta &= G(\eta) \\ \eta &= p^2 + 2p\eta(1-p) + \eta^2(1-p)^2 \\ 0 &= \eta^2(1-p)^2 + [2p(1-p) - 1]\eta + p^2.\end{aligned}$$

From the quadratic formula we have that

$$\begin{aligned}\eta &= \frac{1 - 2p(1 - p) \pm \sqrt{(2p(1 - p) - 1)^2 - 4(1 - p)^2 p^2}}{2(1 - p)^2} \\ &= \frac{1 - 2p(1 - p) \pm (2p - 1)}{2(1 - p)^2}.\end{aligned}$$

Case 1:

$$\begin{aligned}\eta &= \frac{1 - 2p + 2p^2 + 2p - 1}{2(1 - p)^2} \\ &= \frac{p^2}{(1 - p)^2} \\ &= \left(\frac{p}{1 - p}\right)^2.\end{aligned}$$

Case 2:

$$\begin{aligned}\eta &= \frac{1 - 2p + 2p^2 - 2p + 1}{2(1 - p)^2} \\ &= \frac{(p - 1)^2}{(1 - p)^2} \\ &= 1.\end{aligned}$$

We therefore summarize by giving the extinction probability as

$$\eta = \begin{cases} \left(\frac{p}{1-p}\right)^2 & 0 < p \leq \frac{1}{2} \\ \frac{1}{2} & \frac{1}{2} \leq p < 1. \end{cases}$$

### Problem 5 - Dobrow 4.30

R: Simulate the branching process in Problem 3 (Dobrow 4.12). Use your simulation to estimate the extinction probability  $e$ .

### Solution

We simulate the process in R as follows:

```
# branching process simulation
bp_sim <- function(n,k=c(0,1,2),p=c(0.25,0.25,0.5)){
  z_i = 1
  for(i in 1:n){
    if(z_i == 0){
      return(0)
      break
    } else {
      xi = sample(k,z_i,T,p)
      z_i = sum(xi)
    }
  }
}
```

```
    }  
  }  
  if(z_i==0){  
    return(0)  
  } else {  
    return(1)  
  }  
}
```

We can then use Monte-Carlo approximation to estimate the extinction probability:

```
set.seed(49)  
test = replicate(n=1000,bp_sim(n=50))  
mean(test)
```

```
[1] 0.509
```